theories/twoLockMSQ_concurrent_spec.v
@@ -203,10 +203,10 @@ Qed.
 
 Definition queue_invariant (Ψ : val -> iProp Σ) (l_head l_tail : loc) (Q_γ : Qgnames) : iProp Σ :=
 	∃ xs_v, (* Abstract state *)
-	∃ xs xs_rest xs_old (x_head x_tail: (loc * val * loc)), (* Concrete state *)
-	⌜xs = xs_rest ++ [x_head] ++ xs_old⌝ ∗
+	∃ xs xs_queue xs_old (x_head x_tail: (loc * val * loc)), (* Concrete state *)
+	⌜xs = xs_queue ++ [x_head] ++ xs_old⌝ ∗
 	isLL xs ∗
-	⌜proj_val xs_rest = wrap_some xs_v⌝ ∗
+	⌜proj_val xs_queue = wrap_some xs_v⌝ ∗
 	All xs_v Ψ ∗
 	(
 		(* Static *)
@@ -244,10 +244,10 @@ Definition queue_invariant (Ψ : val -> iProp Σ) (l_head l_tail : loc) (Q_γ : 
 
 Definition queue_invariant_simple (Ψ : val -> iProp Σ) (l_head l_tail : loc) (Q_γ : Qgnames) : iProp Σ :=
 	∃ xs_v, (* Abstract state *)
-	∃ xs xs_rest xs_old (x_head x_tail: (loc * val * loc)), (* Concrete state *)
-	⌜xs = xs_rest ++ [x_head] ++ xs_old⌝ ∗
+	∃ xs xs_queue xs_old (x_head x_tail: (loc * val * loc)), (* Concrete state *)
+	⌜xs = xs_queue ++ [x_head] ++ xs_old⌝ ∗
 	isLL xs ∗
-	⌜proj_val xs_rest = wrap_some xs_v⌝ ∗
+	⌜proj_val xs_queue = wrap_some xs_v⌝ ∗
 	All xs_v Ψ ∗
 	(
 		(
@@ -272,8 +272,8 @@ Lemma queue_invariant_equiv_simple : forall Ψ l_head l_tail Q_γ,
 Proof.
 	iIntros (Ψ l_head l_tail Q_γ).
 	iSplit.
-	- iIntros "(%xs_v & %xs & %xs_rest & %xs_old & %x_head & %x_tail & Hxs_split & HisLL_xs & %Hconc_abst_eq & HAll & [H_Static | [H_Enqueue | [H_Dequeue | H_Both]]])"; 
-	iExists xs_v, xs, xs_rest, xs_old, x_head, x_tail; iFrame.
+	- iIntros "(%xs_v & %xs & %xs_queue & %xs_old & %x_head & %x_tail & Hxs_split & HisLL_xs & %Hconc_abst_eq & HAll & [H_Static | [H_Enqueue | [H_Dequeue | H_Both]]])"; 
+	iExists xs_v, xs, xs_queue, xs_old, x_head, x_tail; iFrame.
 	  + iDestruct "H_Static" as "(Hl_head & Hl_tail & HisLast & HTokne & HToknD & HTokUpdated)".
 	  	iSplit; first done.
 		iSplitL "Hl_head HToknD"; first (iLeft; iFrame).
@@ -296,8 +296,8 @@ Proof.
 		* iSplit; first done.
 		  iSplitL "Hl_head HTokD"; first (iRight; iFrame). 
 		  iRight. iFrame. iRight. iFrame.
-	- iIntros "(%xs_v & %xs & %xs_rest & %xs_old & %x_head & %x_tail & Hxs_split & HisLL_xs & %Hconc_abst_eq & HAll & [[Hl_head HToknD] | [Hl_head HTokD]] & [(Hl_tail & HisLast & HToknE & HTokUpdated) | (Hl_tail & HTokE & [[HisLast HTokBefore] | [HisSndLast HTokAfter]])])";
-	iExists xs_v, xs, xs_rest, xs_old, x_head, x_tail; eauto 10 with iFrame.
+	- iIntros "(%xs_v & %xs & %xs_queue & %xs_old & %x_head & %x_tail & Hxs_split & HisLL_xs & %Hconc_abst_eq & HAll & [[Hl_head HToknD] | [Hl_head HTokD]] & [(Hl_tail & HisLast & HToknE & HTokUpdated) | (Hl_tail & HTokE & [[HisLast HTokBefore] | [HisSndLast HTokAfter]])])";
+	iExists xs_v, xs, xs_queue, xs_old, x_head, x_tail; eauto 10 with iFrame.
 Qed.
 
 Definition is_queue (Ψ : val -> iProp Σ) (q : val) (Q_γ: Qgnames) : iProp Σ :=
@@ -390,7 +390,7 @@ Proof.
 	(* Open in Static / Dequeue *)
 	iInv "H_queue_inv" as "H_queue_inv_open".
 	iPoseProof (queue_invariant_equiv_simple Ψ l_head l_tail qg with "H_queue_inv_open") as "H_queue_inv_open".
-	iDestruct "H_queue_inv_open" as "(%xs_v & %xs & %xs_rest & %xs_old & %x_head & %x_tail & >%H_eq_xs & HisLL_xs & >%Hconc_abst_eq & HAll_xs & H_head & [ ( [Hl_tail1 Hl_tail2] & >[%xs_fromtail %H_isLast] & HToknE & HTokUpdated ) | (_ & >HTokE2 & _) ])"; last by iCombine "HTokE HTokE2" gives "%H". (* Impossible: TokE *)
+	iDestruct "H_queue_inv_open" as "(%xs_v & %xs & %xs_queue & %xs_old & %x_head & %x_tail & >%H_eq_xs & HisLL_xs & >%Hconc_abst_eq & HAll_xs & H_head & [ ( [Hl_tail1 Hl_tail2] & >[%xs_fromtail %H_isLast] & HToknE & HTokUpdated ) | (_ & >HTokE2 & _) ])"; last by iCombine "HTokE HTokE2" gives "%H". (* Impossible: TokE *)
 	wp_load.
 	iModIntro.
 	iPoseProof (isLL_and_chain with "HisLL_xs") as "[HisLL_xs #HisLL_chain_xs]".
@@ -401,7 +401,7 @@ Proof.
 	{
 		iNext.
 		iApply queue_invariant_equiv_simple.
-		iExists xs_v, xs, xs_rest, xs_old, x_head, x_tail.
+		iExists xs_v, xs, xs_queue, xs_old, x_head, x_tail.
 		iFrame.
 		do 2 (iSplit; first done).
 		iRight.
@@ -416,7 +416,7 @@ Proof.
 	(* Open in Enqueue / Both : Before *)
 	iInv "H_queue_inv" as "H_queue_inv_open".
 	iPoseProof (queue_invariant_equiv_simple Ψ l_head l_tail qg with "H_queue_inv_open") as "H_queue_inv_open".
-	iDestruct "H_queue_inv_open" as "(%xs_v_2 & %xs_2 & %xs_rest_2 & %xs_old_2 & %x_head_2 & %x_tail_2 & >%H_eq_xs_2 & HisLL_xs_2 & >%Hconc_abst_eq_2 & HAll_xs_2 & H_head & [ ( _ & _ & >HToknE2 & _ ) | (>Hl_tail1 & HTokE & [[>[%xs_fromtail_2 %H_isLast_2] HTokBefore] | [_ >HTokAfter2]]) ])"; 
+	iDestruct "H_queue_inv_open" as "(%xs_v_2 & %xs_2 & %xs_queue_2 & %xs_old_2 & %x_head_2 & %x_tail_2 & >%H_eq_xs_2 & HisLL_xs_2 & >%Hconc_abst_eq_2 & HAll_xs_2 & H_head & [ ( _ & _ & >HToknE2 & _ ) | (>Hl_tail1 & HTokE & [[>[%xs_fromtail_2 %H_isLast_2] HTokBefore] | [_ >HTokAfter2]]) ])"; 
 	[ by iCombine "HToknE HToknE2" gives "%H" | | (* Impossible: ToknE *)
 	  by iCombine "HTokAfter HTokAfter2" gives "%H" ]. (* Impossible: TokAfter *)
 	iCombine "Hl_tail1 Hl_tail2" as "Hl_tail" gives "[_ %Htail_eq]".
@@ -444,7 +444,7 @@ Proof.
 	{
 		iNext.
 		iApply queue_invariant_equiv_simple.
-		iExists (v :: xs_v_2), xs_new, (x_new :: xs_rest_2), xs_old_2, x_head_2, x_tail.
+		iExists (v :: xs_v_2), xs_new, (x_new :: xs_queue_2), xs_old_2, x_head_2, x_tail.
 		iSplit. { iPureIntro. unfold xs_new. cbn. rewrite H_eq_xs_2. auto. }
 		iFrame.
 		iSplit. { iPureIntro. simpl. f_equal. done. }
@@ -463,7 +463,7 @@ Proof.
 	(* Open in Enqueue / Both : After *)
 	iInv "H_queue_inv" as "H_queue_inv_open".
 	iPoseProof (queue_invariant_equiv_simple Ψ l_head l_tail qg with "H_queue_inv_open") as "H_queue_inv_open".
-	iDestruct "H_queue_inv_open" as "(%xs_v_3 & %xs_3 & %xs_rest_3 & %xs_old_3 & %x_head_3 & %x_tail_3 & >%H_eq_xs_3 & HisLL_xs_3 & >%Hconc_abst_eq_3 & HAll_xs_3 & H_head & [ ( _ & _ & >HToknE2 & _ ) | (>Hl_tail1 & HTokE & [[_ >HTokBefore2] | [>(%x_new_2 & %xs_fromtail_3 & %H_isSndLast) HTokAfter]])])"; 
+	iDestruct "H_queue_inv_open" as "(%xs_v_3 & %xs_3 & %xs_queue_3 & %xs_old_3 & %x_head_3 & %x_tail_3 & >%H_eq_xs_3 & HisLL_xs_3 & >%Hconc_abst_eq_3 & HAll_xs_3 & H_head & [ ( _ & _ & >HToknE2 & _ ) | (>Hl_tail1 & HTokE & [[_ >HTokBefore2] | [>(%x_new_2 & %xs_fromtail_3 & %H_isSndLast) HTokAfter]])])"; 
 	[ by iCombine "HToknE HToknE2" gives "%H" | (* Impossible: ToknE *)
 	  by iCombine "HTokBefore HTokBefore2" gives "%H" | ]. (* Impossible: TokBefore *)
 	iCombine "Hl_tail1 Hl_tail2" as "Hl_tail" gives "[_ %Htail_eq2]".
@@ -490,7 +490,7 @@ Proof.
 	{
 		iNext.
 		iApply queue_invariant_equiv_simple.
-		iExists xs_v_3, xs_3, xs_rest_3, xs_old_3, x_head_3, x_new.
+		iExists xs_v_3, xs_3, xs_queue_3, xs_old_3, x_head_3, x_new.
 		iSplit; first done.
 		iFrame.
 		iSplit; first done.
@@ -524,7 +524,7 @@ Proof.
 	(* Open in Static / Enqueue *)
 	iInv "H_queue_inv" as "H_queue_inv_open".
 	iPoseProof (queue_invariant_equiv_simple Ψ l_head l_tail qg with "H_queue_inv_open") as "H_queue_inv_open".
-	iDestruct "H_queue_inv_open" as "(%xs_v & %xs & %xs_rest & %xs_old & %x_head & %x_tail & >%H_eq_xs & H_isLL_xs & >%Hconc_abst_eq & HAll_xs & [ [Hl_head HToknD] | [Hl_head >HTokD2] ] & H_tail)"; 
+	iDestruct "H_queue_inv_open" as "(%xs_v & %xs & %xs_queue & %xs_old & %x_head & %x_tail & >%H_eq_xs & H_isLL_xs & >%Hconc_abst_eq & HAll_xs & [ [Hl_head HToknD] | [Hl_head >HTokD2] ] & H_tail)"; 
 	last by iCombine "HTokD HTokD2" gives "%H". (* Impossible: TokD*)
 	wp_load.
 	iModIntro.
@@ -534,7 +534,7 @@ Proof.
 	iSplitL "Hl_head2 HTokD H_tail H_isLL_xs HAll_xs".
 	{
 		iNext. iApply queue_invariant_equiv_simple.
-		iExists xs_v, xs, xs_rest, xs_old, x_head, x_tail. iFrame.
+		iExists xs_v, xs, xs_queue, xs_old, x_head, x_tail. iFrame.
 		do 2 (iSplit; first done). iRight. done.
 	}
 	wp_let.
@@ -546,7 +546,7 @@ Proof.
 	(* Open in Dequeue / Both *)
 	iInv "H_queue_inv" as "H_queue_inv_open".
 	iPoseProof (queue_invariant_equiv_simple Ψ l_head l_tail qg with "H_queue_inv_open") as "H_queue_inv_open".
-	iDestruct "H_queue_inv_open" as "(%xs_v_2 & %xs_2 & %xs_rest_2 & %xs_old_2 & %x_head_2 & %x_tail_2 & >%H_eq_xs_2 & H_isLL_xs_2 & >%Hconc_abst_eq_2 & HAll_xs_2 & [ [Hl_head >HToknD2] | [>Hl_head2 HTokD] ] & H_tail)";
+	iDestruct "H_queue_inv_open" as "(%xs_v_2 & %xs_2 & %xs_queue_2 & %xs_old_2 & %x_head_2 & %x_tail_2 & >%H_eq_xs_2 & H_isLL_xs_2 & >%Hconc_abst_eq_2 & HAll_xs_2 & [ [Hl_head >HToknD2] | [>Hl_head2 HTokD] ] & H_tail)";
 	first by iCombine "HToknD HToknD2" gives "%H". (* Impossible: ToknD*)
 	iPoseProof (isLL_and_chain with "H_isLL_xs_2") as "[H_isLL_xs_2 #HisLL_chain_xs_2]".
 	iCombine "Hl_head1 Hl_head2" as "Hl_head" gives "[_ %Hhead_eq2]".
@@ -554,11 +554,11 @@ Proof.
 	{
 		iNext.
 		simplify_eq.
-		by iApply (isLL_chain_agree x_head_2 x_head xs_rest_2 xs_old_2 xs_rest xs_old).
+		by iApply (isLL_chain_agree x_head_2 x_head xs_queue_2 xs_old_2 xs_queue xs_old).
 	}
 	subst.
 	(* Case analysis: Is queue empty? *)
-	destruct xs_rest_2 as [| x_tail_2_2 xs_rest_2'].
+	destruct xs_queue_2 as [| x_tail_2_2 xs_queue_2'].
 	- (* Queue is empty. *)
 	  iDestruct "H_isLL_xs_2" as "[H_x_head_out _]".
 	  wp_load.
@@ -582,7 +582,7 @@ Proof.
 	  iApply "HΦ".
 	  by iLeft.
 	- (* Queue is non-empty*)
-	  destruct (exists_first (x_tail_2_2 :: xs_rest_2')) as [x_head_next [xs_rest_2'' Hxs_rest_eq]]; first done.
+	  destruct (exists_first (x_tail_2_2 :: xs_queue_2')) as [x_head_next [xs_rest Hxs_rest_eq]]; first done.
 	  rewrite Hxs_rest_eq.
 	  iAssert (▷(isLL_chain [x_head_next; x_head]))%I as "H_isLL_chain_x_head_next".
 	  {
@@ -601,7 +601,7 @@ Proof.
 	  iSplitL "Hl_head2 H_isLL_xs_2 H_tail HTokD HAll_xs_2".
 	  {
 		iNext. iApply queue_invariant_equiv_simple.
-		iExists xs_v_2, ((xs_rest_2'' ++ [x_head_next]) ++ [x_head] ++ xs_old_2), (xs_rest_2'' ++ [x_head_next]), xs_old_2, x_head, x_tail_2.
+		iExists xs_v_2, ((xs_rest ++ [x_head_next]) ++ [x_head] ++ xs_old_2), (xs_rest ++ [x_head_next]), xs_old_2, x_head, x_tail_2.
 		iFrame. iSplit; first done. iSplit; first by rewrite <- Hxs_rest_eq.  iRight. done.
 	  }
 	  wp_let.
@@ -614,7 +614,7 @@ Proof.
 	  (* Open in Dequeue / Both *)
 	  iInv "H_queue_inv" as "H_queue_inv_open".
 	  iPoseProof (queue_invariant_equiv_simple Ψ l_head l_tail qg with "H_queue_inv_open") as "H_queue_inv_open".
-	  iDestruct "H_queue_inv_open" as "(%xs_v_3 & %xs_3 & %xs_rest_3 & %xs_old_3 & %x_head_3 & %x_tail_3 & >%H_eq_xs_3 & H_isLL_xs_3 & >%Hconc_abst_eq_3 & HAll_xs_3 & [ [Hl_head >HToknD2] | [>Hl_head2 HTokD] ] & H_tail)";
+	  iDestruct "H_queue_inv_open" as "(%xs_v_3 & %xs_3 & %xs_queue_3 & %xs_old_3 & %x_head_3 & %x_tail_3 & >%H_eq_xs_3 & H_isLL_xs_3 & >%Hconc_abst_eq_3 & HAll_xs_3 & [ [Hl_head >HToknD2] | [>Hl_head2 HTokD] ] & H_tail)";
 	  first by iCombine "HToknD HToknD2" gives "%H". (* Impossible ToknD *)
 	  iCombine "Hl_head1 Hl_head2" as "Hl_head" gives "[_ %Hhead_eq3]".
 	  rewrite dfrac_op_own.
@@ -624,18 +624,18 @@ Proof.
 	  iPoseProof (isLL_and_chain with "H_isLL_xs_3") as "[H_isLL_xs_3 #H_isLL_chain_xs_3]".
 	  iAssert (⌜x_head_3 = x_head⌝)%I as "->".
 	  {
-		iApply (isLL_chain_agree x_head_3 x_head xs_rest_3 xs_old_3 xs_rest xs_old); by simplify_eq.
+		iApply (isLL_chain_agree x_head_3 x_head xs_queue_3 xs_old_3 xs_queue xs_old); by simplify_eq.
 	  }
 	  subst.
-	  (* Sync up xs_rest_2 with xs_rest_3 *)
-	  destruct xs_rest_3 as [|x_tail_3_2 xs_rest_3'].
-	  { (* Impossible case. xs_rest_3 must contain at least one element. *)
+	  (* Sync up xs_queue_3 with xs_queue_2 *)
+	  destruct xs_queue_3 as [|x_tail_3_2 xs_queue_3'].
+	  { (* Impossible case. xs_queue_3 must contain at least one element. *)
 		iDestruct "H_isLL_xs_3" as "[H_x_head_3_null _]".
 		iCombine "H_x_head_3_null H_x_head_next_out" gives "[_ %Hcontra]".
 		simplify_eq.
 	  }
-	  destruct (exists_first (x_tail_3_2 :: xs_rest_3')) as [x_head_next_3 [xs_rest_3'' Hxs_rest_eq_3]]; first done.
-	  rewrite Hxs_rest_eq_3.
+	  destruct (exists_first (x_tail_3_2 :: xs_queue_3')) as [x_head_next_3 [xs_rest' Hxs_rest_eq']]; first done.
+	  rewrite Hxs_rest_eq'.
 	  rewrite <- app_assoc. rewrite <- app_assoc.
 	  iAssert (⌜x_head_next = x_head_next_3⌝)%I as "->"; first by iApply isLL_chain_agree_next.
 	  destruct xs_v_3 as [|x_v xs'_v_3]; 
@@ -643,17 +643,17 @@ Proof.
 	  destruct (exists_first (x_v :: xs'_v_3)) as [x_head_next_val [xs_val_rest Hxs_val_rest_eq]]; first done.
 	  rewrite Hxs_val_rest_eq in Hconc_abst_eq_3.
 	  rewrite Hxs_val_rest_eq.
-	  rewrite Hxs_rest_eq_3 in Hconc_abst_eq_3.
-	  rewrite (proj_val_split xs_rest_3'' [x_head_next_3]) in Hconc_abst_eq_3.
+	  rewrite Hxs_rest_eq' in Hconc_abst_eq_3.
+	  rewrite (proj_val_split xs_rest' [x_head_next_3]) in Hconc_abst_eq_3.
 	  rewrite (wrap_some_split xs_val_rest [x_head_next_val]) in Hconc_abst_eq_3.
 	  simpl in Hconc_abst_eq_3.
-	  apply (list_last_eq (proj_val xs_rest_3'') (wrap_some xs_val_rest) (n_val x_head_next_3) (InjRV x_head_next_val)) in Hconc_abst_eq_3 as [Hxs_rest_val_eq Hx_head_next_eq].
+	  apply (list_last_eq (proj_val xs_rest') (wrap_some xs_val_rest) (n_val x_head_next_3) (InjRV x_head_next_val)) in Hconc_abst_eq_3 as [Hxs_rest_val_eq Hx_head_next_eq].
 	  iPoseProof (All_split with "HAll_xs_3") as "[HAll_xs_val_rest [Hx_head_next_val_Ψ _]]".
 	  (* Close in Static / Enqueue *)
 	  iSplitL "Hl_head H_tail HToknD H_isLL_xs_3 HAll_xs_val_rest".
 	  {
 		iNext. iApply queue_invariant_equiv_simple.
-		iExists xs_val_rest, (xs_rest_3'' ++ [x_head_next_3] ++ [x_head] ++ xs_old_3), xs_rest_3'', ([x_head] ++ xs_old_3), x_head_next_3, x_tail_3.
+		iExists xs_val_rest, (xs_rest' ++ [x_head_next_3] ++ [x_head] ++ xs_old_3), xs_rest', ([x_head] ++ xs_old_3), x_head_next_3, x_tail_3.
 		iFrame. iSplit; first done.
 		iSplit; first done.
 		iLeft.
